\section*{6.4}

Prove Theorem 6.2.10

\vspace{5mm}
\hrule
\vspace{5mm}
\noindent\textbf{Theorem 6.2.10}

Let $X_1, \cdots, X_n$ be iid observations from a pdf or pmf $f(x\mid\theta)$, which belongs to an exponential family given by:

\[
	f(x\mid\theta) = h(x)c(\theta)\exp\left( \sum_{i=1}^k w_i(\theta)t_i(x) \right),
\]

where $\theta = (\theta_1, \cdots, \theta_d), d \leq k$. Then

\[T(\vec{X}) = \left( \sum_{j=1}^n t_1(X_j), \cdots, \sum_{j=1}^n t_k(X_j)\right)\]

is a sufficient statistic for $\theta$.

\vspace{5mm}
\hrule
\vspace{5mm}

\noindent We'll be leveraging the factorization theorem for this proof.

We begin by writing out the joint pdf of the exponential family.

\begin{align*}
	f(\vec{x}\mid\theta) &= \prod_{i=1}^n h(x_i)c(\theta)\exp\left( \sum_{j=1}^k w_j(\theta)t_j(x_i) \right) \\
	&= c(\theta)^n \left( \prod_{i=1}^n h(x_i) \right) \cdot \exp\left( \sum_{j=1}^k w_j(\theta) \sum_{i=1}^n t_j(x_i) \right) &\text{(Distribute product)} \\
	&=\left( \prod_{i=1}^n h(x_i) \right) \cdot  c(\theta)^n \cdot \exp\left( \sum_{j=1}^k w_j(\theta) \sum_{i=1}^n t_j(x_i) \right) &\text{(Rearrange)}\\ 
\end{align*}

Giving us 

\vspace{-5mm}
\begin{align*}
	g(T(\vec{x}) \mid \theta) &=  c(\theta)^n \cdot \exp\left( \sum_{j=1}^k w_j(\theta) \sum_{i=1}^n t_j(x_i) \right) \\
	h(\vec{x}) &= \prod_{i=1}^n h(x_i)
\end{align*}

Therefore,

\[
	T(\vec{x}) = \left( \sum_{i=1}^n t_1(x_i), \cdots, \sum_{i=1}^n t_k(x_i)  \right)
\]

is a sufficient statistic for $\theta$ by the factorization theorem.
